Tweaked the relation a bit in order to be able to prove completeness w.r.t. contextual approximation

theories/L6_PCPS/ctx_approx.v
@@ -1,68 +1,75 @@
 Require Import Coq.Arith.Arith Coq.NArith.BinNat Coq.Lists.List Coq.omega.Omega
         Coq.Relations.Relations Coq.Classes.RelationClasses.
 Require Import cps ctx eval identifiers.
-
+Import ListNotations.
 
 Definition empty_env := M.empty val.
 
 Open Scope ctx_scope. 
 
-(** Contextual approximation w.r.t. R *)
-Definition ctx_approx (R : relation val) : relation exp :=
+(** Contextual approximation *)
+Definition ctx_approx : relation exp :=
   fun e1 e2 =>
     forall C i v1, eval.bstep_e empty_env (C |[ e1 ]|) v1 i ->
-              exists v2 j, eval.bstep_e empty_env (C |[ e2 ]|) v2 j /\
-                      R v1 v2.
+              exists v2 j, eval.bstep_e empty_env (C |[ e2 ]|) v2 j.
 
-(** Contextual equivalence w.r.t. R *)
-Definition ctx_equiv (R : relation val) : relation exp :=
-  fun e1 e2 => ctx_approx R e1 e2 /\ ctx_approx R e2 e1.
+(** Contextual equivalence *)
+Definition ctx_equiv : relation exp :=
+  fun e1 e2 => ctx_approx e1 e2 /\ ctx_approx e2 e1.
 
-
-Lemma ctx_approx_trans (R : relation val) :
-  Transitive R ->
-  Transitive (ctx_approx R).
+Lemma ctx_approx_trans :
+  Transitive ctx_approx.
 Proof. 
-  intros Ht. intros x y z H1 H2 C i v1 Hstep.
-  edestruct H1 as [v2 [j2 [Hstep2 Hr2]]]; eauto. 
-  edestruct H2 as [v3 [j3 [Hstep3 Hr3]]]; eauto.
+  intros x y z H1 H2 C i v1 Hstep.
+  edestruct H1 as [v2 [j2 Hstep2]]; eauto. 
 Qed.
 
-Lemma ctx_approx_refl (R : relation val) :
-  Reflexive R ->
-  Reflexive (ctx_approx R).
+Lemma ctx_approx_refl :
+  Reflexive ctx_approx.
 Proof. 
-  intros Ht. intros x C i v1 Hstep.
+  intros x C i v1 Hstep.
   repeat split; eauto.
 Qed.
 
-Lemma ctx_equiv_equiv (R : relation val) :
-  Transitive R ->
-  Reflexive R ->
-  Equivalence (ctx_equiv R).
+Lemma ctx_equiv_equiv :
+  Equivalence ctx_equiv.
 Proof.
-  intros Ht Hr. constructor.
+  constructor.
   - split; apply ctx_approx_refl; eauto.
   - split; eapply H.
   - intros x y z [H1 H2] [H3 H4]; split; eapply ctx_approx_trans; eauto.
 Qed.
 
-Lemma preord_exp_sound (R : relation val) e1 e2 :
-  inclusion _ (fun v1 v2 => forall k, preord_val k v1 v2) R ->
+Lemma preord_exp_sound e1 e2 :
   (forall k rho1 rho2, preord_env_P (occurs_free e1) k rho1 rho2 ->
                   preord_exp k (e1, rho1) (e2, rho2)) ->
-  ctx_approx R e1 e2.
+  ctx_approx e1 e2.
 Proof.
-  intros Hincl Hyp C i v1 Hstep.
+  intros Hyp C i v1 Hstep.
   assert (Hyp' := Hyp).
   eapply (preord_exp_compat i empty_env empty_env C) in Hyp;
   [| now eapply preord_env_P_refl ].
   edestruct Hyp as [v2 [c2 [Hstep2 Hpre2]]]; eauto.
-  repeat eexists; eauto. 
-  eapply Hincl. intros k.
-  eapply (preord_exp_compat (k + i) empty_env empty_env C) in Hyp';
-  [| now eapply preord_env_P_refl ].
-  edestruct Hyp' as [v2' [c2' [Hstep2' Hpre2']]]; [| eassumption |]; try omega.
-  eapply bstep_e_deterministic in Hstep2'; [| now apply Hstep2 ].
-  inv Hstep2'. eapply preord_val_monotonic. now apply Hpre2'. omega.
+Qed.
+
+Definition x : var := 1%positive.
+Definition y : var := 2%positive.
+
+Definition tau : type := 1%positive.
+Definition c : tag := 1%positive.
+
+Definition stuck : exp :=
+  Econstr x tau c [] (
+  Econstr y tau c [] (
+  Eapp x [y])).
+
+Lemma stuck_gets_stuck rho :
+  ~ (exists v c, bstep_e rho stuck v c).
+Proof.
+  intros [v [c H]]. inv H. inv H8.
+  inv H10. inv H7. inv H9.
+  - rewrite M.gso, M.gss in H2. inv H2.
+    intros Hc. inv Hc.
+  - rewrite M.gso, M.gss in H1. inv H1.
+    intros Hc. inv Hc.
 Qed.
